fixed bugs in loop handling for infeasible code detection.

gravy/src/org/gravy/loopunwinding/AbstractLoopUnwinding.java
@@ -4,10 +4,15 @@ import java.util.HashMap;
 import java.util.HashSet;
 import java.util.LinkedList;
 
+import org.gravy.GlobalsCache;
 import org.gravy.Options;
 
+import boogie.ProgramFactory;
+import boogie.ast.Attribute;
 import boogie.controlflow.BasicBlock;
 import boogie.controlflow.CfgProcedure;
+import boogie.controlflow.expression.CfgBooleanLiteral;
+import boogie.controlflow.statement.CfgAssertStatement;
 
 /**
  * @author schaef
@@ -16,20 +21,22 @@ public abstract class AbstractLoopUnwinding {
 
 	public static void unwindeLoops(CfgProcedure proc) {
 		AbstractLoopUnwinding unwinder = null;
-		if (Options.v().getUnwindings()<0) {
+		if (Options.v().getUnwindings() < 0) {
 			unwinder = new HavocOnlyUnwinding(proc);
 		} else {
 			unwinder = new SimpleUnwinding(proc, Options.v().getUnwindings());
 		}
 		unwinder.unwind();
 	}
-	
+
 	/**
 	 * Boogie procedure
 	 */
 	protected CfgProcedure proc;
 
 	protected int maxUnwinding = 0;
+
+	protected boolean dontVerifyClones = false;
 	
 	/**
 	 * C-tor
@@ -41,83 +48,86 @@ public abstract class AbstractLoopUnwinding {
 		this.proc = proc;
 	}
 
+	
+	
 	/**
 	 * Unwinds the loops
 	 */
 	public abstract void unwind();
-	
-	
+
 	/**
-	 * Eliminates a loop by removing all BasicBlocks
-	 * that must reach the loop head. 
-	 * This works for all sorts of loops but probably 
-	 * generates much larger programs than the typical 
-	 * loop elimination that we would do for normal while 
-	 * loops (namely just removing the enitre body). 
+	 * Eliminates a loop by removing all BasicBlocks that must reach the loop
+	 * head. This works for all sorts of loops but probably generates much
+	 * larger programs than the typical loop elimination that we would do for
+	 * normal while loops (namely just removing the enitre body).
+	 * 
 	 * @param loop
 	 */
 	private void eliminateDoWhileLoop(LoopInfo loop) {
-		//identify all blocks that can exit the loop.
+		// identify all blocks that can exit the loop.
 		LinkedList<BasicBlock> todo = new LinkedList<BasicBlock>();
-		for (BasicBlock b:   loop.loopExit) {
+		for (BasicBlock b : loop.loopExit) {
 			for (BasicBlock pre : b.getPredecessors()) {
 				if (loop.loopBody.contains(pre)) {
 					todo.add(pre);
 				}
-			}			
+			}
 		}
-		
-		//now find all blocks that connect the
-		//loop entry to a loop exit
+
+		// now find all blocks that connect the
+		// loop entry to a loop exit
 		LinkedList<BasicBlock> connectedToExit = new LinkedList<BasicBlock>();
 		while (!todo.isEmpty()) {
 			BasicBlock b = todo.pop();
 			connectedToExit.add(b);
-			if (b!=loop.loopHead) {
+			if (b != loop.loopHead) {
 				for (BasicBlock pre : b.getPredecessors()) {
 					if (!todo.contains(pre)) {
 						todo.add(pre);
 					}
 				}
-			}			
+			}
 		}
-		
+
 		for (BasicBlock b : loop.loopBody) {
 			if (connectedToExit.contains(b)) {
 				for (BasicBlock s : new HashSet<BasicBlock>(b.getSuccessors())) {
-					if (!loop.loopExit.contains(s) && !connectedToExit.contains(s) ) {
+					if (!loop.loopExit.contains(s)
+							&& !connectedToExit.contains(s)) {
 						b.disconnectFromSuccessor(s);
 					}
- 				}
+				}
 			} else {
 				for (BasicBlock s : new HashSet<BasicBlock>(b.getSuccessors())) {
 					b.disconnectFromSuccessor(s);
-				}				
+				}
 			}
-		}		
+		}
 	}
-	
+
 	private void eliminateWhileDoLoop(LoopInfo loop) {
-		//remove the entire loop and connect the head only
-		//to the exit.
+		// remove the entire loop and connect the head only
+		// to the exit.
 		for (BasicBlock b : loop.loopBody) {
-			if (b==loop.loopHead) continue;
+			if (b == loop.loopHead)
+				continue;
 			for (BasicBlock s : new HashSet<BasicBlock>(b.getSuccessors())) {
 				if (!loop.loopBody.contains(s)) {
 					b.disconnectFromSuccessor(s);
 				}
 			}
 		}
-		for (BasicBlock b : new HashSet<BasicBlock>(loop.loopHead.getSuccessors())) {
+		for (BasicBlock b : new HashSet<BasicBlock>(
+				loop.loopHead.getSuccessors())) {
 			if (loop.loopBody.contains(b)) {
 				loop.loopHead.disconnectFromSuccessor(b);
 			}
-		}		
+		}
 	}
-	
+
 	protected void eliminate(LoopInfo loop) {
-		//check if the we have a while-do / for loop
-		//or a do-while loop.
+		// check if the we have a while-do / for loop
+		// or a do-while loop.
 		boolean isDoWhile = true;
 		for (BasicBlock b : loop.loopHead.getSuccessors()) {
 			if (!loop.loopBody.contains(b)) {
@@ -125,7 +135,7 @@ public abstract class AbstractLoopUnwinding {
 				break;
 			}
 		}
-		
+
 		if (isDoWhile) {
 			System.err.println("Do-While Loop found");
 			eliminateDoWhileLoop(loop);
@@ -134,62 +144,78 @@ public abstract class AbstractLoopUnwinding {
 			eliminateWhileDoLoop(loop);
 		}
 	}
-	
+
 	protected void unwind(LoopInfo loop, int unwindings) {
 		for (LoopInfo nest : loop.nestedLoops) {
 			unwind(nest, unwindings);
 		}
 
-		if (unwindings<=0) {
+		if (unwindings <= 0) {
 			eliminate(loop);
 			return;
 		}
-		
-		//first unwind the nested loops.
-		//clone the loop once and add it before the actual loop.
+
+		// first unwind the nested loops.
+		// clone the loop once and add it before the actual loop.
 		HashMap<BasicBlock, BasicBlock> clonemap = new HashMap<BasicBlock, BasicBlock>();
-		//clone the loopbody
+		// clone the loopbody
 		BasicBlock cloneHead = null;
 		for (BasicBlock b : loop.loopBody) {
-			BasicBlock clone = b.clone("iter"+(this.maxUnwinding- unwindings));
-			if (b==loop.loopHead) {
+			BasicBlock clone = b.clone("iter"
+					+ (this.maxUnwinding - unwindings));
+			if (b == loop.loopHead) {
 				cloneHead = clone;
 			}
+			// TODO: not sure if this is the right condition. Eventually,
+			// if we want to do abstract unwinding, we have to make
+			// the clones NoCode blocks.
+			if (dontVerifyClones) {
+				ignoreInVerification(clone);
+			}
+			
 			clonemap.put(b, clone);
 		}
 
-		if (cloneHead==null) {
+		if (cloneHead == null) {
 			throw new RuntimeException("No loop head found during unwinding.");
 		}
-		//now redirect the predecessors of the loop head to the 
-		//head of the clone.
+		// now redirect the predecessors of the loop head to the
+		// head of the clone.
 		for (BasicBlock b : loop.loopEntries) {
 			b.disconnectFromSuccessor(loop.loopHead);
 			b.connectToSuccessor(cloneHead);
 		}
- 		
-		//fix the successors of the cloned nodes.
+
+		// fix the successors of the cloned nodes.
 		for (BasicBlock b : loop.loopBody) {
 			BasicBlock clone = clonemap.get(b);
 			for (BasicBlock s : new HashSet<BasicBlock>(b.getSuccessors())) {
-				if (clonemap.containsKey(s)) {					
+				if (clonemap.containsKey(s)) {
 					clone.connectToSuccessor(clonemap.get(s));
 				} else {
-					//add the missing edge that was not cloned
+					// add the missing edge that was not cloned
 					clone.connectToSuccessor(s);
 				}
 			}
 		}
-				
-		//now redirect all back edges to the original loop head.
+
+		// now redirect all back edges to the original loop head.
 		for (BasicBlock b : loop.loopingPred) {
 			BasicBlock clone = clonemap.get(b);
 			clone.disconnectFromSuccessor(cloneHead);
-			clone.connectToSuccessor(loop.loopHead);	
+			clone.connectToSuccessor(loop.loopHead);
 		}
-		
+
 		loop.UpdateLoopEntries();
-		
-		unwind(loop, unwindings-1);		
-	}	
+
+		unwind(loop, unwindings - 1);
+	}
+	
+	private void ignoreInVerification(BasicBlock clone) {
+		ProgramFactory pf = GlobalsCache.v().getProgramFactory();
+		clone.addStatement(new CfgAssertStatement(null,
+				new Attribute[] { pf.mkNoCodeAttribute() },
+				new CfgBooleanLiteral(null, pf.getBoolType(), true)));	
+	}
+	
 }
