gravy/src/org/gravy/loopunwinding/HavocOnlyUnwinding.java
@@ -1,8 +1,6 @@
 package org.gravy.loopunwinding;
 
-import java.util.HashMap;
 import java.util.HashSet;
-import java.util.LinkedList;
 import java.util.List;
 
 import util.Log;
@@ -31,6 +29,7 @@ public class HavocOnlyUnwinding extends AbstractLoopUnwinding {
 		super(proc);
 		this.proc = proc;
 		this.maxUnwinding=1;
+		this.dontVerifyClones=true;
 	}
 
 	@Override
@@ -56,105 +55,14 @@ public class HavocOnlyUnwinding extends AbstractLoopUnwinding {
 			b.addStatement(computeHavocStatement(loop), true);
 		}
 		
-		//disconnectLoopingControlFlow(loop);
-		
 		if (loop.loopExit.size()==0) {
 			Log.error("Loop has no exit! LoopHead "+loop.loopHead.getLabel());
 		}
 		
 		unwind(loop,this.maxUnwinding);
-		//eliminate(loop);
 		
 	}
 	
-	private void disconnectLoopingControlFlow(LoopInfo l) {
-		
-		/*
-		 * Here, we eliminate the looping executions of the loop.
-		 * This is a bit tricky as we cannot assume that we have a structured
-		 * loop of the form while(x) B which we could easily transform into
-		 * a conditional choice. 
-		 * Instead, we have to identify all blocks in the loop body that only occur
-		 * on looping executions and remove them from the program. As result, we obtain
-		 */
-		
-		//first remove the looping edges
-		for (BasicBlock b : l.loopingPred) {
-			b.disconnectFromSuccessor(l.loopHead);
-		}
-				
-		
-		//now find the part of the loop that can leave
-		//the loop body
-		LinkedList<BasicBlock> todo = new LinkedList<BasicBlock>();   
-		todo.addAll(l.loopExit); 
-		LinkedList<BasicBlock> done = new LinkedList<BasicBlock>();		
-		
-		HashSet<BasicBlock> nonLoopingBody = new HashSet<BasicBlock>();
-		while (!todo.isEmpty()) {
-			BasicBlock current = todo.removeLast();
-			done.add(current);
-			for (BasicBlock pred : current.getPredecessors()) {
-				if (l.loopBody.contains(pred) && !done.contains(pred) && !todo.contains(pred)) {
-					nonLoopingBody.add(pred);
-					todo.add(pred);
-				}
-			}			
-		}
-		
-		//now clone the part of the loop body that must leave the loop and
-		//redirect the back edge to this clone
-		HashMap<BasicBlock, BasicBlock> clonemap = new HashMap<BasicBlock, BasicBlock>();		
-		for (BasicBlock b : nonLoopingBody) {
-			clonemap.put(b, b.clone("clone"));
-		}
-		//clone the loophead as well
-		clonemap.put(l.loopHead, l.loopHead.clone("clone"));
-
-		//update the edges of the cloned blocks
-		for (BasicBlock b : nonLoopingBody) {
-			BasicBlock clone = clonemap.get(b);
-			for (BasicBlock pre : new HashSet<BasicBlock>(b.getPredecessors())) {				
-				if (clonemap.containsKey(pre)) {
-					clonemap.get(pre).connectToSuccessor(clone);
-				}
-			}
-			for (BasicBlock suc : new HashSet<BasicBlock>(b.getSuccessors())) {
-				if (l.loopBody.contains(suc)) {					
-					if (clonemap.containsKey(suc)) {
-						clone.connectToSuccessor(clonemap.get(suc));
-					} 
-				} else {
-					//if the successor is outside of the loop, we have to refresh 
-					//the reference, because the successor does not yet know its cloned
-					//predecessor
-					clone.connectToSuccessor(suc);
-				}
-			}
-		}
-		{
-			BasicBlock clone = clonemap.get(l.loopHead);
-			//redo the same thing for the loop head
-			for (BasicBlock suc : new HashSet<BasicBlock>(l.loopHead.getSuccessors())) {
-				if (l.loopBody.contains(suc)) {					
-					if (clonemap.containsKey(suc)) {
-						clone.connectToSuccessor(clonemap.get(suc));
-					} 
-				} else {
-					//if the successor is outside of the loop, we have to refresh 
-					//the reference, because the successor does not yet know its cloned
-					//predecessor
-					clone.connectToSuccessor(suc);
-				}
-			}
-		}
-		
-		for (BasicBlock b : l.loopingPred) {
-			b.connectToSuccessor(clonemap.get(l.loopHead));
-		}
-			
-		
-	}
 
 	private CfgHavocStatement computeHavocStatement(LoopInfo l) {
 		HashSet<CfgVariable> havocedVars = new HashSet<CfgVariable>();
